src/Rewriter/ArithWithCasts.v
@@ -1,0 +1,37 @@
+Require Import Crypto.Language.
+Require Import Crypto.LanguageWf.
+Require Import Crypto.RewriterProofsTactics.
+Require Import Crypto.RewriterRulesProofs.
+
+Module Compilers.
+  Import Language.Compilers.
+  Import Language.Compilers.defaults.
+  Import LanguageWf.Compilers.
+  Import RewriterProofsTactics.Compilers.RewriteRules.GoalType.
+  Import RewriterProofsTactics.Compilers.RewriteRules.Tactic.
+
+  Module Import RewriteRules.
+    Section __.
+      Definition VerifiedRewriterArithWithCasts : VerifiedRewriter.
+      Proof using All. make_rewriter false arith_with_casts_rewrite_rules_proofs. Defined.
+
+      Definition RewriteArithWithCasts {t} := Eval hnf in @Rewrite VerifiedRewriterArithWithCasts t.
+
+      Lemma Wf_RewriteArithWithCasts {t} e (Hwf : Wf e) : Wf (@RewriteArithWithCasts t e).
+      Proof. now apply VerifiedRewriterArithWithCasts. Qed.
+
+      Lemma Interp_gen_RewriteArithWithCasts {cast_outside_of_range t} e (Hwf : Wf e)
+        : expr.Interp (@ident.gen_interp cast_outside_of_range) (@RewriteArithWithCasts t e)
+          == expr.Interp (@ident.gen_interp cast_outside_of_range) e.
+      Proof. now apply VerifiedRewriterArithWithCasts. Qed.
+
+      Lemma Interp_RewriteArithWithCasts {t} e (Hwf : Wf e) : Interp (@RewriteArithWithCasts t e) == Interp e.
+      Proof. apply Interp_gen_RewriteArithWithCasts; assumption. Qed.
+    End __.
+  End RewriteRules.
+
+  Module Export Hints.
+    Hint Resolve Wf_RewriteArithWithCasts : wf.
+    Hint Rewrite @Interp_gen_RewriteArithWithCasts @Interp_RewriteArithWithCasts : interp.
+  End Hints.
+End Compilers.
