src/Rewriter/ToFancy.v
@@ -1,0 +1,45 @@
+Require Import Coq.ZArith.ZArith.
+Require Import Crypto.Language.
+Require Import Crypto.LanguageWf.
+Require Import Crypto.RewriterProofsTactics.
+Require Import Crypto.RewriterRulesProofs.
+
+Module Compilers.
+  Import Language.Compilers.
+  Import Language.Compilers.defaults.
+  Import LanguageWf.Compilers.
+  Import RewriterProofsTactics.Compilers.RewriteRules.GoalType.
+  Import RewriterProofsTactics.Compilers.RewriteRules.Tactic.
+
+  Module Import RewriteRules.
+    Section __.
+      Context (invert_low invert_high : Z (*log2wordmax*) -> Z -> @option Z)
+              (Hlow : forall s v v', invert_low s v = Some v' -> v = Z.land v' (2^(s/2)-1))
+              (Hhigh : forall s v v', invert_high s v = Some v' -> v = Z.shiftr v' (s/2)).
+
+      Definition VerifiedRewriterToFancy : VerifiedRewriter.
+      Proof using All. make_rewriter false fancy_rewrite_rules_proofs. Defined.
+
+      Definition RewriteToFancy {t} : Expr t -> Expr t.
+      Proof using invert_low invert_high.
+        let v := (eval hnf in (@Rewrite VerifiedRewriterToFancy t)) in exact v.
+      Defined.
+
+      Lemma Wf_RewriteToFancy {t} e (Hwf : Wf e) : Wf (@RewriteToFancy t e).
+      Proof using All. now apply VerifiedRewriterToFancy. Qed.
+
+      Lemma Interp_gen_RewriteToFancy {cast_outside_of_range t} e (Hwf : Wf e)
+        : expr.Interp (@ident.gen_interp cast_outside_of_range) (@RewriteToFancy t e)
+          == expr.Interp (@ident.gen_interp cast_outside_of_range) e.
+      Proof using All. now apply VerifiedRewriterToFancy. Qed.
+
+      Lemma Interp_RewriteToFancy {t} e (Hwf : Wf e) : Interp (@RewriteToFancy t e) == Interp e.
+      Proof using All. apply Interp_gen_RewriteToFancy; assumption. Qed.
+    End __.
+  End RewriteRules.
+
+  Module Export Hints.
+    Hint Resolve Wf_RewriteToFancy : wf.
+    Hint Rewrite @Interp_gen_RewriteToFancy @Interp_RewriteToFancy : interp.
+  End Hints.
+End Compilers.
