src/RewriterProofsTactics.v
@@ -1,0 +1,107 @@
+Require Import Crypto.Language.
+Require Import Crypto.LanguageInversion.
+Require Import Crypto.LanguageWf.
+Require Import Crypto.UnderLetsProofs.
+Require Import Crypto.GENERATEDIdentifiersWithoutTypesProofs.
+Require Import Crypto.Rewriter.
+Require Import Crypto.RewriterWf1.
+Require Import Crypto.RewriterWf2.
+Require Import Crypto.RewriterInterpProofs1.
+Require Import Crypto.Util.Tactics.CacheTerm.
+Require Import Crypto.Util.Tactics.ConstrFail.
+
+Module Compilers.
+  Import LanguageWf.Compilers.
+  Import GENERATEDIdentifiersWithoutTypes.Compilers.
+  Import GENERATEDIdentifiersWithoutTypesProofs.Compilers.
+  Import Rewriter.Compilers.RewriteRules.
+  Import RewriterWf1.Compilers.RewriteRules.
+  Import RewriterWf2.Compilers.RewriteRules.
+  Import RewriterInterpProofs1.Compilers.RewriteRules.
+  Import Rewriter.Compilers.RewriteRules.GoalType.
+  Import RewriterWf1.Compilers.RewriteRules.GoalType.
+  Import RewriterWf1.Compilers.RewriteRules.WfTactics.GoalType.
+  Import RewriterWf1.Compilers.RewriteRules.InterpTactics.GoalType.
+  Import RewriterWf1.Compilers.RewriteRules.WfTactics.Tactic.
+  Import RewriterWf1.Compilers.RewriteRules.InterpTactics.Tactic.
+
+  Module Import RewriteRules.
+    Definition VerifiedRewriter_of_Rewriter
+               (R : RewriterT)
+               (RWf : Wf_GoalT R)
+               (RInterp : Interp_GoalT R)
+               (RProofs : PrimitiveHList.hlist
+                            (@snd bool Prop)
+                            (List.skipn (dummy_count (Rewriter_data R)) (rewrite_rules_specs (Rewriter_data R))))
+    : VerifiedRewriter.
+    Proof.
+      simple refine
+             (let HWf := _ in
+              let HInterp_gen := _ in
+              @Build_VerifiedRewriter (@Rewriter.Compilers.RewriteRules.GoalType.Rewrite R) HWf HInterp_gen (HInterp_gen _));
+        [ | clear HWf ]; intros.
+      all: abstract (
+               rewrite Rewrite_eq; cbv [Make.Rewrite]; rewrite rewrite_head_eq, all_rewrite_rules_eq;
+               first [ apply Compile.Wf_Rewrite; [ | assumption ];
+                       let wf_do_again := fresh "wf_do_again" in
+                       (intros ? ? ? ? wf_do_again ? ?);
+                       eapply @Compile.wf_assemble_identifier_rewriters;
+                       eauto using
+                             pattern.Raw.ident.to_typed_invert_bind_args, pattern.ident.eta_ident_cps_correct
+                         with nocore;
+                       try reflexivity
+                     | eapply Compile.InterpRewrite; [ | assumption ];
+                       intros; eapply Compile.interp_assemble_identifier_rewriters with (pident_to_typed:=@pattern.ident.to_typed);
+                       eauto using
+                             pattern.Raw.ident.to_typed_invert_bind_args, pattern.ident.eta_ident_cps_correct, pattern.ident.unify_to_typed,
+                       @ident.gen_interp_Proper, eq_refl
+                         with nocore ]).
+    Defined.
+
+    Ltac make_VerifiedRewriter R RWf RInterp RProofs :=
+      let res := (eval hnf in (@VerifiedRewriter_of_Rewriter R RWf RInterp RProofs)) in
+      let res := lazymatch res with
+                 | context Res[@Build_VerifiedRewriter ?R]
+                   => let t := fresh "t" in
+                      let R' := fresh in
+                      let R' := constr:(fun t
+                                        => match R t return _ with
+                                           | R' => ltac:(let v := (eval hnf in R') in exact v)
+                                           end) in
+                      context Res[@Build_VerifiedRewriter R']
+                 end in
+      res.
+
+    Ltac Build_Rewriter include_interp specs_proofs :=
+      let specs := lazymatch type of specs_proofs with
+                   | PrimitiveHList.hlist (@snd bool Prop) ?specs => specs
+                   | ?T
+                     => let expected_type := uconstr:(PrimitiveHList.hlist (@snd bool Prop) ?[specs]) in
+                        constr_fail_with ltac:(fun _ => fail 1 "Invalid type for specs_proofs:" T "Expected:" expected_type)
+                   end in
+      let R_name := fresh "Rewriter_data" in
+      let R := Build_RewriterT include_interp specs in
+      let R := cache_term R R_name in
+      let Rwf := fresh "Rewriter_Wf" in
+      let Rwf := cache_proof_with_type_by (Wf_GoalT R) ltac:(idtac; prove_good ()) Rwf in
+      let RInterp := fresh "Rewriter_Interp" in
+      let RInterp := cache_proof_with_type_by (Interp_GoalT R) ltac:(idtac; prove_interp_good ()) RInterp in
+      make_VerifiedRewriter R Rwf RInterp specs_proofs.
+
+    Module Export GoalType.
+      Export RewriterWf1.Compilers.RewriteRules.GoalType.
+    End GoalType.
+
+    Module Export Tactic.
+      Module Export Settings.
+        Export Rewriter.Compilers.RewriteRules.Tactic.Settings.
+      End Settings.
+
+      Ltac make_rewriter include_interp specs_proofs :=
+        let res := Build_Rewriter include_interp specs_proofs in refine res.
+
+      Tactic Notation "make_rewriter" constr(include_interp) constr(specs_proofs) :=
+        make_rewriter include_interp specs_proofs.
+    End Tactic.
+  End RewriteRules.
+End Compilers.
